Typed transforms

theories/erasure/Transforms.v
@@ -43,3 +43,137 @@ Final Obligation.
   cbn. intros.
   destruct enable_unsafe as [[] ? ? ?]=> //.
 Qed.
+
+
+Section Dearging.
+  Import Optimize OptimizeCorrectness.
+
+  Definition dearg (p : (option dearg_set × ExAst.global_env) * EAst.term) : ExAst.global_env * EAst.term :=
+    match p.1.1 with
+    | Some masks => ((dearg_env masks p.1.2), dearg_term masks p.2)
+    | None => (p.1.2, p.2)
+    end.
+
+  Program Definition dearging_transform (efl := EWellformed.all_env_flags) cf :
+    Transform.t _ _  EAst.term EAst.term _ _ (eval_typed_eprogram_masks EWcbvEval.opt_wcbv_flags) (eval_typed_eprogram EWcbvEval.opt_wcbv_flags) :=
+    {| name := "dearging";
+      transform p _ := dearg p ;
+      pre p := post_dearging_checks efl cf p;
+      post p := wf_eprogram efl (ExAst.trans_env p.1, p.2) /\ EEtaExpandedFix.expanded_eprogram (ExAst.trans_env p.1, p.2) ;
+      obseq p hp p' v v' := v' = (dearg (p.1, v)).2 |}.
+  Next Obligation.
+  Proof.
+    cbn. intros.
+    unfold dearg.
+    destruct p. rewrite H.
+    destruct check_dearging_precond eqn:eqp; cbn -[ExAst.trans_env] => //.
+    destruct input as [[masks env] t]. cbn -[ExAst.trans_env Optimize.dearg_env] in *.
+    subst masks. destruct H0 as [wf exp].
+    eapply check_dearging_precond_spec in eqp. intuition.
+    - split; cbn.
+      unfold dearg_env.
+      eapply wf_glob_debox.
+      eapply wf_glob_dearg; eauto.
+      eapply wf.
+      rewrite /dearg_env. rewrite -trans_env_debox.
+      eapply wellformed_dearg; eauto.
+      eapply wf.
+    - rewrite /dearg_env -trans_env_debox. split; cbn.
+      eapply expanded_dearg_env; tea. apply exp.
+      eapply EEtaExpandedFix.isEtaExp_expanded, expanded_dearg; eauto.
+      apply EEtaExpandedFix.expanded_isEtaExp, exp.
+  Qed.
+  Final Obligation.
+    cbn. intros. red.
+    intros p v [he [wfe exp]]. unfold eval_typed_eprogram_masks.
+    intros [ev].
+    unfold dearg. rewrite he.
+    destruct (check_dearging_precond) as [masks|] eqn:cpre.
+    * eapply (ExtractionCorrectness.extract_correct_gen' _ _ _ masks cf.(overridden_masks) cf.(do_trim_const_masks) cf.(do_trim_ctor_masks)) in ev as ev'.
+      destruct ev' as [ev'].
+      eexists. split. red. sq. cbn. exact ev'. auto.
+      - destruct wfe. now eapply EWellformed.wellformed_closed_env.
+      - destruct wfe. now eapply EWellformed.wellformed_closed.
+      - move: cpre. unfold check_dearging_precond. destruct EGlobalEnv.closed_env => //.
+        destruct ExtractionCorrectness.compute_masks => //.
+        destruct (_ && _) => //. congruence.
+      - move: cpre. rewrite /check_dearging_precond.
+        destruct EGlobalEnv.closed_env => //.
+        destruct ExtractionCorrectness.compute_masks => //.
+        destruct valid_cases eqn:vc => //. cbn.
+        destruct is_expanded => //. now intros [= ->].
+      - move: cpre. rewrite /check_dearging_precond.
+        destruct EGlobalEnv.closed_env => //.
+        destruct ExtractionCorrectness.compute_masks => //.
+        destruct valid_cases eqn:vc => //. cbn.
+        destruct is_expanded eqn:ise => //. now intros [= ->].
+    * exists v. cbn. split => //.
+  Qed.
+End Dearging.
+
+Program Definition dearging_transform_mapping (cf : ETransform.dearging_config) :
+  Transform.t _ _ _ _ _ _ (eval_typed_eprogram_masks_mapping EWcbvEval.opt_wcbv_flags) (eval_typed_eprogram_mapping EWcbvEval.opt_wcbv_flags)  :=
+  let tr := (dearging_transform cf) in
+ {| name := name tr;
+    pre p := EReorderCstrs.wf_inductives_mapping (ExAst.trans_env p.2.1.2) p.1 /\ pre tr p.2 ;
+    transform p hp := let nhs := proj2 hp in (p.1, transform tr p.2 nhs) ;
+    post p := EReorderCstrs.wf_inductives_mapping (ExAst.trans_env p.2.1) p.1 /\ post tr p.2;
+    obseq p hp p' := obseq tr p.2 (proj2 hp) p'.2 |}.
+Next Obligation.
+Proof.
+  cbn.
+  split => //.
+  2:{ now unshelve eapply (correctness (dearging_transform cf)). }
+  destruct p.
+  move: H; rewrite /EReorderCstrs.wf_inductives_mapping; solve_all.
+  move: H; rewrite /EReorderCstrs.wf_inductive_mapping. destruct x as [ind [na tags]].
+  rewrite /dearg. destruct input.2.1.1 => //.
+  rewrite /OptimizeCorrectness.dearg_env.
+  rewrite /EGlobalEnv.lookup_inductive /EGlobalEnv.lookup_minductive /=.
+  rewrite !OptimizeCorrectness.lookup_env_trans_env.
+  rewrite OptimizeCorrectness.lookup_env_debox_env_types option_map_two /=.
+  rewrite OptimizeCorrectness.lookup_env_dearg_env option_map_two /=.
+  destruct ExAst.lookup_env => //=; destruct g => //=.
+  rewrite !nth_error_map option_map_two /=.
+  rewrite /Optimize.dearg_mib /=. destruct Optimize.get_mib_masks => //=.
+  rewrite !nth_error_mapi.
+  1-2:destruct nth_error eqn:hnth => //=; len.
+  intros _. destruct o => //=. destruct p => //.
+Qed.
+Final Obligation.
+Proof.
+  intros cf p v pr ev. cbn.
+  now unshelve eapply (preservation (dearging_transform cf)).
+Qed.
+
+Program Definition typed_transform_pipeline {guard : abstract_guard_impl}
+  (efl := EWellformed.all_env_flags) econf
+  : Transform.t _ _ _ _ _ _
+   (eval_typed_eprogram_mapping EWcbvEval.default_wcbv_flags)
+   (eval_typed_eprogram_mapping EWcbvEval.opt_wcbv_flags) :=
+
+   remove_match_on_box_typed_transform_mapping (wcon := eq_refl) (hastrel := eq_refl) (hastbox := eq_refl)
+    (fl := EWcbvEval.default_wcbv_flags) ▷
+   (* Check if the preconditions for dearging are valid, otherwise dearging will be the identity *)
+   dearging_checks_transform_mapping econf.(dearging_config) (hastrel := eq_refl) (hastbox := eq_refl) ▷
+   dearging_transform_mapping econf.(dearging_config).
+Next Obligation.
+  program_simpl.
+Qed.
+Next Obligation.
+  program_simpl.
+Qed.
+Next Obligation.
+  program_simpl.
+Qed.
+Next Obligation.
+  program_simpl.
+Qed.
+Next Obligation.
+  intros. cbn.
+  apply H.
+Qed.
+Final Obligation.
+  cbn. intros.
+  apply H.
+Qed.
